{-# OPTIONS --without-K --rewriting #-}
module rewriting.examples.CastSafeLogic where

open import Agda.Primitive using (lzero)
open import Data.List using (List; []; _∷_; length)
open import Data.Nat
open import Data.Nat.Induction
open import Data.Bool using (true; false) renaming (Bool to 𝔹)
open import Data.Nat.Properties
open import Data.Product using (_,_;_×_; proj₁; proj₂; Σ-syntax; ∃-syntax)
open import Data.Unit using (⊤; tt)
open import Data.Unit.Polymorphic renaming (⊤ to ⊤ᵖ; tt to ttᵖ)
open import Data.Vec using (Vec) renaming ([] to []̌; _∷_ to _∷̌_)
open import Data.Empty using (⊥; ⊥-elim)
open import Data.Sum using (_⊎_; inj₁; inj₂)
open import Induction using (RecStruct)
open import Induction.WellFounded as WF
open import Data.Product.Relation.Binary.Lex.Strict
  using (×-Lex; ×-wellFounded; ×-preorder)
open import Relation.Binary using (Rel)
open import Relation.Binary.PropositionalEquality as Eq
  using (_≡_; _≢_; refl; sym; cong; subst; trans)
open import Relation.Nullary using (¬_; Dec; yes; no)
open import Sig
open import Var
open import rewriting.examples.Cast
open import rewriting.examples.CastLogRelLogic

{-# REWRITE sub-var #-}

compatibility-var : ∀ {Γ A x}
  → Γ ∋ x ⦂ A
    -----------
  → Γ ⊨ ` x ⦂ A
compatibility-var {Γ}{A}{x} ∋x k γ 𝓖Γγk =
  let Vγx = lemma-𝓖 Γ γ k 𝓖Γγk ∋x in
  Val⇒Exp {A}{⟪ γ ⟫ (` x)} k Vγx

compatible-nat : ∀{Γ}{n : ℕ} → Γ ⊨ ($ n) ⦂ ($ₜ ′ℕ)
compatible-nat {Γ}{n} k γ 𝓖Γγk = Val⇒Exp{$ₜ ′ℕ} k (G k)
    where G : ∀ k → 𝓥⟦ $ₜ ′ℕ ⟧ ($ n) k
          G zero = tt
          G (suc k) = subst (λ X → X) (sym (V-base{k}{′ℕ}{′ℕ}{n})) refl

compatible-bool : ∀{Γ}{b : 𝔹} → Γ ⊨ ($ b) ⦂ ($ₜ ′𝔹)
compatible-bool {Γ}{b} k γ 𝓖Γγk = Val⇒Exp{$ₜ ′𝔹} k (G k)
    where G : ∀ k → 𝓥⟦ $ₜ ′𝔹 ⟧ ($ b) k
          G zero = tt
          G (suc k) = subst (λ X → X) (sym (V-base{k}{′𝔹}{′𝔹}{b})) refl

compatible-app : ∀{Γ}{A}{B}{L}{M}
    → Γ ⊨ L ⦂ (A ⇒ B)
    → Γ ⊨ M ⦂ A
      -------------------
    → Γ ⊨ L · M ⦂ B
compatible-app {Γ}{A}{B}{L}{M} ⊨L ⊨M k γ 𝓖Γγk = Goal
    where
    𝓔L : 𝓔⟦ A ⇒ B ⟧ (⟪ γ ⟫ L ) k
    𝓔L = ⊨L k γ 𝓖Γγk

    𝓔M : 𝓔⟦ A ⟧ (⟪ γ ⟫ M ) k
    𝓔M = ⊨M k γ 𝓖Γγk

    Goal2 : (V : Term) (r : ⟪ γ ⟫ L —↠ V) → 𝓔⟦ B ⟧ (V · ⟪ γ ⟫ M) (k + len r)
    Goal2 V L→V = 𝓔-frame{B}{{!!} ·□}{⟪ γ ⟫ M}{k + len L→V} {!!}

    Goal : 𝓔⟦ B ⟧ (⟪ γ ⟫ (L · M)) k
    Goal = 𝓔-frame{B}{□· (⟪ γ ⟫ M)}{⟪ γ ⟫ L}{k} Goal2
